examples/n_german/nGerman.thy
@@ -28,22 +28,11 @@ definition n_RecvGntE :: "nat \<Rightarrow> rule" where
     assign (Para ''Cache.State'' i, Const E) ||
     assign (Para ''Chan2.Cmd'' i, Const Empty)"
 
-lemma symRecvGntE:
+lemma RecvGntE:
   "symParamRule N n_RecvGntE"
+  "wellFormedStatement N (act (n_RecvGntE i))"
+  "absTransfRule M (n_RecvGntE i) = (if i \<le> M then n_RecvGntE i else chaos \<triangleright> skip)"
   unfolding n_RecvGntE_def symParamRule_def by auto
-
-lemma absRecvGntE:
-  "absTransfForm M (pre (n_RecvGntE i)) =
-    (if i > M then dontCareForm
-     else IVar (Para ''Chan2.Cmd'' i) =\<^sub>f Const GntE)"
-  by (auto simp add: n_RecvGntE_def)
-
-lemma absRecvGntEAct:
-  "absTransfStatement2 M (act (n_RecvGntE i)) =
-    (if i > M then skip
-     else assign (Para ''Cache.State'' i, Const (enum ''control'' ''E'')) ||
-          assign (Para ''Chan2.Cmd'' i, Const (enum ''control'' ''Empty'')))"
-  unfolding n_RecvGntE_def by auto
 
 definition n_RecvGntS :: "nat \<Rightarrow> rule" where
   "n_RecvGntS i \<equiv>
@@ -52,22 +41,11 @@ definition n_RecvGntS :: "nat \<Rightarrow> rule" where
     assign (Para ''Cache.State'' i, Const S) ||
     assign (Para ''Chan2.Cmd'' i, Const Empty)"
 
-lemma symRecvGntS:
+lemma RecvGntS:
   "symParamRule N n_RecvGntS"
+  "wellFormedStatement N (act (n_RecvGntS i))"
+  "absTransfRule M (n_RecvGntS i) = (if i \<le> M then n_RecvGntS i else chaos \<triangleright> skip)"
   unfolding n_RecvGntS_def symParamRule_def by auto
-
-lemma absRecvGntS:
-  "absTransfForm M (pre (n_RecvGntS i)) =
-    (if i > M then dontCareForm
-     else IVar (Para ''Chan2.Cmd'' i) =\<^sub>f Const GntS)"
-  by (auto simp add: n_RecvGntS_def)
-
-lemma absRecvGntSAct:
-  "absTransfStatement2 M (act (n_RecvGntS i)) =
-    (if i > M then skip
-     else assign (Para ''Cache.State'' i, Const (enum ''control'' ''S'')) ||
-          assign (Para ''Chan2.Cmd'' i, Const (enum ''control'' ''Empty'')))"
-  unfolding n_RecvGntS_def by auto
 
 definition n_SendGntE :: "nat \<Rightarrow> nat \<Rightarrow> rule" where
   "n_SendGntE N i \<equiv>
@@ -82,45 +60,27 @@ definition n_SendGntE :: "nat \<Rightarrow> nat \<Rightarrow> rule" where
     assign (Ident ''ExGntd'', Const true) ||
     assign (Ident ''CurCmd'', Const Empty)"
 
-lemma symSendGntE:
+definition n_SendGntE_abs :: "nat \<Rightarrow> rule" where
+  "n_SendGntE_abs M \<equiv>
+    IVar (Ident ''CurCmd'') =\<^sub>f Const ReqE \<and>\<^sub>f
+    IVar (Ident ''CurPtr'') =\<^sub>f Const (index (M+1)) \<and>\<^sub>f
+    IVar (Ident ''ExGntd'') =\<^sub>f Const false \<and>\<^sub>f
+    (\<forall>\<^sub>fj. IVar (Para ''ShrSet'' j) =\<^sub>f Const false) M
+   \<triangleright>
+    assign (Ident ''ExGntd'', Const true) ||
+    assign (Ident ''CurCmd'', Const Empty)"
+
+lemma wellFormedSendGntE:
   "symParamRule N (n_SendGntE N)"
+  "wellFormedStatement N (act (n_SendGntE N i))"
   unfolding n_SendGntE_def
-  apply (rule symParamRuleI)
-  apply (auto intro!: symParamFormAnd symParamFormForall)
+  apply (auto intro!: symParamRuleI symParamFormAnd symParamFormForall)
   unfolding symParamForm_def symParamForm2_def symParamStatement_def by auto
 
 lemma absSendGntE:
-  assumes "M \<le> N"
-  shows
-  "absTransfForm M (pre (n_SendGntE N i)) =
-    (if i > M then
-       IVar (Ident ''CurCmd'') =\<^sub>f Const ReqE \<and>\<^sub>f
-       IVar (Ident ''CurPtr'') =\<^sub>f Const (index (M+1)) \<and>\<^sub>f
-       IVar (Ident ''ExGntd'') =\<^sub>f Const false \<and>\<^sub>f
-       (\<forall>\<^sub>fj. IVar (Para ''ShrSet'' j) =\<^sub>f Const false) M
-     else
-       IVar (Ident ''CurCmd'') =\<^sub>f Const ReqE \<and>\<^sub>f
-       IVar (Ident ''CurPtr'') =\<^sub>f Const (index i) \<and>\<^sub>f
-       IVar (Para ''Chan2.Cmd'' i) =\<^sub>f Const Empty \<and>\<^sub>f
-       IVar (Ident ''ExGntd'') =\<^sub>f Const false \<and>\<^sub>f
-       (\<forall>\<^sub>fj. IVar (Para ''ShrSet'' j) =\<^sub>f Const false) M)"
-  unfolding n_SendGntE_def using assms by auto
-
-lemma absSendGntEAct:
-  "absTransfStatement2 M (act (n_SendGntE N i)) =
-    (if i > M then
-       assign (Ident ''ExGntd'', Const true) ||
-       assign (Ident ''CurCmd'', Const Empty)
-     else
-       assign (Para ''Chan2.Cmd'' i, Const GntE) ||
-       assign (Para ''ShrSet'' i, Const true) ||
-       assign (Ident ''ExGntd'', Const true) ||
-       assign (Ident ''CurCmd'', Const Empty))"
-  unfolding n_SendGntE_def by auto
-
-lemma SendGntEWellForm:
-  "wellFormedStatement N (act (n_SendGntE N i))"
-  unfolding n_SendGntE_def by auto
+  "M \<le> N \<Longrightarrow> absTransfRule M (n_SendGntE N i) =
+     (if i \<le> M then n_SendGntE M i else n_SendGntE_abs M)"
+  unfolding n_SendGntE_def n_SendGntE_abs_def by auto
 
 definition n_SendGntS :: "nat \<Rightarrow> rule" where
   "n_SendGntS i \<equiv>
@@ -133,38 +93,24 @@ definition n_SendGntS :: "nat \<Rightarrow> rule" where
     assign (Para ''ShrSet'' i, Const true) ||
     assign (Ident ''CurCmd'', Const Empty)"
 
-lemma symSendGntS:
+definition n_SendGntS_abs :: "nat \<Rightarrow> rule" where
+  "n_SendGntS_abs M \<equiv>
+    IVar (Ident ''CurCmd'') =\<^sub>f Const ReqS \<and>\<^sub>f
+    IVar (Ident ''CurPtr'') =\<^sub>f Const (index (M+1)) \<and>\<^sub>f
+    IVar (Ident ''ExGntd'') =\<^sub>f Const false
+   \<triangleright>
+    assign (Ident ''CurCmd'', Const Empty)"
+
+lemma wellFormedSendGntS:
   "symParamRule N n_SendGntS"
+  "wellFormedStatement N (act (n_SendGntS i))"
   unfolding n_SendGntS_def
-  apply (rule symParamRuleI)
-  by (auto simp add: symParamForm_def symParamStatement_def)
+  by (auto intro!: symParamRuleI simp add: symParamForm_def symParamStatement_def)
 
 lemma absSendGntS:
-  "absTransfForm M (pre (n_SendGntS i)) =
-    (if i > M then
-       IVar (Ident ''CurCmd'') =\<^sub>f Const ReqS \<and>\<^sub>f
-       IVar (Ident ''CurPtr'') =\<^sub>f Const (index (M+1)) \<and>\<^sub>f
-       IVar (Ident ''ExGntd'') =\<^sub>f Const false
-     else
-       IVar (Ident ''CurCmd'') =\<^sub>f Const ReqS \<and>\<^sub>f
-       IVar (Ident ''CurPtr'') =\<^sub>f Const (index i) \<and>\<^sub>f
-       IVar (Para ''Chan2.Cmd'' i) =\<^sub>f Const Empty \<and>\<^sub>f
-       IVar (Ident ''ExGntd'') =\<^sub>f Const false)"
-  unfolding n_SendGntS_def by auto
-
-lemma absSendGntSAct:
-  "absTransfStatement2 M (act (n_SendGntS i)) =
-    (if i > M then
-       assign (Ident ''CurCmd'', Const Empty)
-     else
-       assign (Para ''Chan2.Cmd'' i, Const GntS) ||
-       assign (Para ''ShrSet'' i, Const true) ||
-       assign (Ident ''CurCmd'', Const Empty))"
-  unfolding n_SendGntS_def by auto
-
-lemma SendGntSWellForm:
-  "wellFormedStatement N (act (n_SendGntS i))"
-  unfolding n_SendGntS_def by auto
+  "M \<le> N \<Longrightarrow> absTransfRule M (n_SendGntS i) =
+    (if i \<le> M then n_SendGntS i else n_SendGntS_abs M)"
+  unfolding n_SendGntS_def n_SendGntS_abs_def by auto
 
 definition n_RecvInvAck1 :: "nat \<Rightarrow> rule" where
   "n_RecvInvAck1 i \<equiv>
@@ -176,34 +122,18 @@ definition n_RecvInvAck1 :: "nat \<Rightarrow> rule" where
     assign (Para ''ShrSet'' i, Const false) ||
     assign (Ident ''ExGntd'', Const false)"
 
-lemma symRecvInvAck1:
-  "symParamRule N (n_RecvInvAck1)"
-  unfolding n_RecvInvAck1_def unfolding symParamRule_def by auto
+definition n_RecvInvAck1_abs :: rule where
+  "n_RecvInvAck1_abs \<equiv>
+    \<not>\<^sub>f IVar (Ident ''CurCmd'') =\<^sub>f Const Empty \<and>\<^sub>f
+    IVar (Ident ''ExGntd'') =\<^sub>f Const true
+   \<triangleright>
+    assign (Ident ''ExGntd'', Const false)"
 
-lemma absRecvInvAck1:
-  "absTransfForm M (pre (n_RecvInvAck1 i)) =
-    (if i > M then
-       \<not>\<^sub>f IVar (Ident ''CurCmd'') =\<^sub>f Const Empty \<and>\<^sub>f
-       IVar (Ident ''ExGntd'') =\<^sub>f Const true
-     else
-       IVar (Para ''Chan3.Cmd'' i) =\<^sub>f Const InvAck \<and>\<^sub>f
-       \<not>\<^sub>f IVar (Ident ''CurCmd'') =\<^sub>f Const Empty \<and>\<^sub>f
-       IVar (Ident ''ExGntd'') =\<^sub>f Const true)"
-  unfolding n_RecvInvAck1_def by auto
-
-lemma absRecvInvAck1Act:
-  "absTransfStatement2 M (act (n_RecvInvAck1 i)) =
-    (if i > M then
-       assign (Ident ''ExGntd'', Const false)
-     else
-       assign (Para ''Chan3.Cmd'' i, Const Empty) ||
-       assign (Para ''ShrSet'' i, Const false) ||
-       assign (Ident ''ExGntd'', Const false))"
-  unfolding n_RecvInvAck1_def by auto
-
-lemma RecvInvAck1WellForm:
+lemma RecvInvAck1:
+  "symParamRule N n_RecvInvAck1"
   "wellFormedStatement N (act (n_RecvInvAck1 i))"
-  unfolding n_RecvInvAck1_def by auto
+  "absTransfRule M (n_RecvInvAck1 i) = (if i \<le> M then n_RecvInvAck1 i else n_RecvInvAck1_abs)"
+  unfolding n_RecvInvAck1_def n_RecvInvAck1_abs_def symParamRule_def by auto
 
 definition n_RecvInvAck2 :: "nat \<Rightarrow> rule" where
   "n_RecvInvAck2 i \<equiv>
@@ -214,33 +144,18 @@ definition n_RecvInvAck2 :: "nat \<Rightarrow> rule" where
     assign (Para ''Chan3.Cmd'' i, Const Empty) ||
     assign (Para ''ShrSet'' i, Const false)"
 
-lemma symRecvInvAck2:
+definition n_RecvInvAck2_abs :: rule where
+  "n_RecvInvAck2_abs \<equiv>
+    \<not>\<^sub>f IVar (Ident ''CurCmd'') =\<^sub>f Const Empty \<and>\<^sub>f
+    \<not>\<^sub>f IVar (Ident ''ExGntd'') =\<^sub>f Const true
+   \<triangleright>
+    skip"
+
+lemma RecvInvAck2:
   "symParamRule N n_RecvInvAck2"
-  unfolding n_RecvInvAck2_def symParamRule_def by auto
-
-lemma absRecvInvAck2:
-  "absTransfForm M (pre (n_RecvInvAck2 i)) =
-    (if i > M then
-       \<not>\<^sub>f IVar (Ident ''CurCmd'') =\<^sub>f Const Empty \<and>\<^sub>f
-       \<not>\<^sub>f IVar (Ident ''ExGntd'') =\<^sub>f Const true
-     else
-       IVar (Para ''Chan3.Cmd'' i) =\<^sub>f Const InvAck \<and>\<^sub>f
-       \<not>\<^sub>f IVar (Ident ''CurCmd'') =\<^sub>f Const Empty \<and>\<^sub>f
-       \<not>\<^sub>f IVar (Ident ''ExGntd'') =\<^sub>f Const true)"
-  unfolding n_RecvInvAck2_def by auto
-
-lemma absRecvInvAck2Act:
-  "absTransfStatement2 M (act (n_RecvInvAck2 i)) =
-    (if i > M then
-       skip
-     else
-       assign (Para ''Chan3.Cmd'' i, Const Empty) ||
-       assign (Para ''ShrSet'' i, Const false))"
-  unfolding n_RecvInvAck2_def by auto
-
-lemma RecvInvAck2WellForm:
   "wellFormedStatement N (act (n_RecvInvAck2 i))"
-  unfolding n_RecvInvAck2_def by auto
+  "absTransfRule M (n_RecvInvAck2 i) = (if i \<le> M then n_RecvInvAck2 i else n_RecvInvAck2_abs)"
+  unfolding n_RecvInvAck2_def n_RecvInvAck2_abs_def symParamRule_def by auto
 
 definition n_SendInvAck1 :: "nat \<Rightarrow> rule" where
   "n_SendInvAck1 i \<equiv>
@@ -252,33 +167,11 @@ definition n_SendInvAck1 :: "nat \<Rightarrow> rule" where
     assign (Para ''Chan3.Cmd'' i, Const InvAck) ||
     assign (Para ''Cache.State'' i, Const I)"
 
-lemma symSendInvAck1:
+lemma SendInvAck1:
   "symParamRule N n_SendInvAck1"
-  unfolding n_SendInvAck1_def symParamRule_def by auto
-
-lemma absSendInvAck1:
-  "absTransfForm M (pre (n_SendInvAck1 i)) =
-    (if i > M then
-       dontCareForm
-     else
-       IVar (Para ''Chan2.Cmd'' i) =\<^sub>f Const Inv \<and>\<^sub>f
-       IVar (Para ''Chan3.Cmd'' i) =\<^sub>f Const Empty \<and>\<^sub>f
-       IVar (Para ''Cache.State'' i) =\<^sub>f Const E)"
-  unfolding n_SendInvAck1_def by auto
-
-lemma absSendInvAck1Act:
-  "absTransfStatement2 M (act (n_SendInvAck1 i)) =
-    (if i > M then
-       skip
-     else
-       assign (Para ''Chan2.Cmd'' i, Const Empty) ||
-       assign (Para ''Chan3.Cmd'' i, Const InvAck) ||
-       assign (Para ''Cache.State'' i, Const I))"
-  unfolding n_SendInvAck1_def by auto
-
-lemma SendInvAck1WellForm:
   "wellFormedStatement N (act (n_SendInvAck1 i))"
-  unfolding n_SendInvAck1_def by auto
+  "absTransfRule M (n_SendInvAck1 i) = (if i \<le> M then n_SendInvAck1 i else chaos \<triangleright> skip)"
+  unfolding n_SendInvAck1_def symParamRule_def by auto
 
 definition n_SendInvAck2 :: "nat \<Rightarrow> rule" where
   "n_SendInvAck2 i \<equiv>
@@ -290,33 +183,11 @@ definition n_SendInvAck2 :: "nat \<Rightarrow> rule" where
     assign (Para ''Chan3.Cmd'' i, Const InvAck) ||
     assign (Para ''Cache.State'' i, Const I)"
 
-lemma symSendInvAck2:
+lemma SendInvAck2:
   "symParamRule N n_SendInvAck2"
-  unfolding n_SendInvAck2_def symParamRule_def by auto
-
-lemma absSendInvAck2:
-  "absTransfForm M (pre (n_SendInvAck2 i)) =
-    (if i > M then
-       dontCareForm
-     else
-       IVar (Para ''Chan2.Cmd'' i) =\<^sub>f Const Inv \<and>\<^sub>f
-       IVar (Para ''Chan3.Cmd'' i) =\<^sub>f Const Empty \<and>\<^sub>f
-       \<not>\<^sub>f IVar (Para ''Cache.State'' i) =\<^sub>f Const E)"
-  unfolding n_SendInvAck2_def by auto
-
-lemma absSendInvAck2Act:
-  "absTransfStatement2 M (act (n_SendInvAck2 i)) =
-    (if i > M then
-       skip
-     else
-       assign (Para ''Chan2.Cmd'' i, Const Empty) ||
-       assign (Para ''Chan3.Cmd'' i, Const InvAck) ||
-       assign (Para ''Cache.State'' i, Const I))"
-  unfolding n_SendInvAck2_def by auto
-
-lemma SendInvAck2WellForm:
   "wellFormedStatement N (act (n_SendInvAck2 i))"
-  unfolding n_SendInvAck2_def by auto
+  "absTransfRule M (n_SendInvAck2 i) = (if i \<le> M then n_SendInvAck2 i else chaos \<triangleright> skip)"
+  unfolding n_SendInvAck2_def symParamRule_def by auto
 
 definition n_SendInv1 :: "nat \<Rightarrow> rule" where
   "n_SendInv1 i \<equiv>
@@ -327,32 +198,17 @@ definition n_SendInv1 :: "nat \<Rightarrow> rule" where
     assign (Para ''Chan2.Cmd'' i, Const Inv) ||
     assign (Para ''InvSet'' i, Const false)"
 
-lemma symSendInv1:
+definition n_SendInv1_abs :: rule where
+  "n_SendInv1_abs \<equiv>
+    IVar (Ident ''CurCmd'') =\<^sub>f Const ReqE
+   \<triangleright>
+    skip"
+
+lemma SendInv1:
   "symParamRule N n_SendInv1"
-  unfolding n_SendInv1_def symParamRule_def by auto
-
-lemma absSendInv1:
-  "absTransfForm M (pre (n_SendInv1 i)) =
-    (if i > M then
-       IVar (Ident ''CurCmd'') =\<^sub>f Const ReqE
-     else
-       IVar (Para ''Chan2.Cmd'' i) =\<^sub>f Const Empty \<and>\<^sub>f
-       IVar (Para ''InvSet'' i) =\<^sub>f Const true \<and>\<^sub>f
-       IVar (Ident ''CurCmd'') =\<^sub>f Const ReqE)"
-  unfolding n_SendInv1_def by auto
-
-lemma absSendInv1Act:
-  "absTransfStatement2 M (act (n_SendInv1 i)) =
-    (if i > M then
-       skip
-     else
-       assign (Para ''Chan2.Cmd'' i, Const Inv) ||
-       assign (Para ''InvSet'' i, Const false))"
-  unfolding n_SendInv1_def by auto
-
-lemma SendInv1WellForm:
   "wellFormedStatement N (act (n_SendInv1 i))"
-  unfolding n_SendInv1_def by auto
+  "absTransfRule M (n_SendInv1 i) = (if i \<le> M then n_SendInv1 i else n_SendInv1_abs)"
+  unfolding n_SendInv1_def n_SendInv1_abs_def symParamRule_def by auto
 
 definition n_SendInv2 :: "nat \<Rightarrow> rule" where
   "n_SendInv2 i \<equiv>
@@ -364,34 +220,18 @@ definition n_SendInv2 :: "nat \<Rightarrow> rule" where
     assign (Para ''Chan2.Cmd'' i, Const Inv) ||
     assign (Para ''InvSet'' i, Const false)"
 
-lemma symSendInv2:
+definition n_SendInv2_abs :: rule where
+  "n_SendInv2_abs \<equiv>
+    IVar (Ident ''CurCmd'') =\<^sub>f Const ReqS \<and>\<^sub>f
+    IVar (Ident ''ExGntd'') =\<^sub>f Const true
+   \<triangleright>
+    skip"
+
+lemma SendInv2:
   "symParamRule N n_SendInv2"
-  unfolding n_SendInv2_def symParamRule_def by auto
-
-lemma absSendInv2:
-  "absTransfForm M (pre (n_SendInv2 i)) =
-    (if i > M then
-       IVar (Ident ''CurCmd'') =\<^sub>f Const ReqS \<and>\<^sub>f
-       IVar (Ident ''ExGntd'') =\<^sub>f Const true
-     else
-       IVar (Para ''Chan2.Cmd'' i) =\<^sub>f Const Empty \<and>\<^sub>f
-       IVar (Para ''InvSet'' i) =\<^sub>f Const true \<and>\<^sub>f
-       IVar (Ident ''CurCmd'') =\<^sub>f Const ReqS \<and>\<^sub>f
-       IVar (Ident ''ExGntd'') =\<^sub>f Const true)"
-  unfolding n_SendInv2_def by auto
-
-lemma absSendInv2Act:
-  "absTransfStatement2 M (act (n_SendInv2 i)) =
-    (if i > M then
-       skip
-     else
-       assign (Para ''Chan2.Cmd'' i, Const (enum ''control'' ''Inv'')) ||
-       assign (Para ''InvSet'' i, Const (boolV False)))"
-  unfolding n_SendInv2_def by auto
-
-lemma SendInv2WellForm:
   "wellFormedStatement N (act (n_SendInv2 i))"
-  unfolding n_SendInv2_def by auto
+  "absTransfRule M (n_SendInv2 i) = (if i \<le> M then n_SendInv2 i else n_SendInv2_abs)"
+  unfolding n_SendInv2_def n_SendInv2_abs_def symParamRule_def by auto
 
 definition n_RecvReqE :: "nat \<Rightarrow> nat \<Rightarrow> rule" where
   "n_RecvReqE N i \<equiv>
@@ -403,40 +243,24 @@ definition n_RecvReqE :: "nat \<Rightarrow> nat \<Rightarrow> rule" where
     assign (Para ''Chan1.Cmd'' i, Const Empty) ||
     forallStm (\<lambda>j. assign (Para ''InvSet'' j, IVar (Para ''ShrSet'' j))) N"
 
-lemma symRecvReqE:
+definition n_RecvReqE_abs :: "nat \<Rightarrow> rule" where
+  "n_RecvReqE_abs M \<equiv>
+    IVar (Ident ''CurCmd'') =\<^sub>f Const Empty
+   \<triangleright>
+    assign (Ident ''CurCmd'', Const ReqE) ||
+    assign (Ident ''CurPtr'', Const (index (M+1))) ||
+    forallStm (\<lambda>j. assign (Para ''InvSet'' j, IVar (Para ''ShrSet'' j))) M"
+
+lemma wellFormedReqE:
   "symParamRule N (n_RecvReqE N)"
+  "wellFormedStatement N (act (n_RecvReqE N i))"
   unfolding n_RecvReqE_def
-  apply (rule symParamRuleI)
-  subgoal unfolding symParamForm_def by auto
-  subgoal apply (auto intro!: symParamStatementParallel symParamStatementForall)
-    unfolding symParamStatement_def symParamStatement2_def mutualDiffVars_def by auto
-  done
+  apply (auto intro!: symParamRuleI symParamStatementParallel symParamStatementForall)
+  unfolding symParamForm_def symParamStatement_def symParamStatement2_def mutualDiffVars_def by auto
 
 lemma absRecvReqE:
-  "absTransfForm M (pre (n_RecvReqE N i)) =
-    (if i > M then
-       IVar (Ident ''CurCmd'') =\<^sub>f Const Empty
-     else
-       IVar (Ident ''CurCmd'') =\<^sub>f Const Empty \<and>\<^sub>f
-       IVar (Para ''Chan1.Cmd'' i) =\<^sub>f Const ReqE)"
-  unfolding n_RecvReqE_def by auto
-
-lemma absRecvReqEAct:
-  "absTransfStatement2 M (act (n_RecvReqE N i)) =
-    (if i > M then
-       assign (Ident ''CurCmd'', Const ReqE) ||
-       assign (Ident ''CurPtr'', Const (index (M+1))) ||
-       forallStm (\<lambda>j. assign (Para ''InvSet'' j, IVar (Para ''ShrSet'' j))) M
-     else
-       assign (Ident ''CurCmd'', Const ReqE) ||
-       assign (Ident ''CurPtr'', Const (index i)) ||
-       assign (Para ''Chan1.Cmd'' i, Const Empty) ||
-       forallStm (\<lambda>j. assign (Para ''InvSet'' j, IVar (Para ''ShrSet'' j))) M)"
-  unfolding n_RecvReqE_def by auto
-
-lemma RecvReqEWellForm:
-  "wellFormedStatement N (act (n_RecvReqE N i))"
-  unfolding n_RecvReqE_def by auto
+  "absTransfRule M (n_RecvReqE N i) = (if i \<le> M then n_RecvReqE M i else n_RecvReqE_abs M)"
+  unfolding n_RecvReqE_def n_RecvReqE_abs_def by auto
 
 definition n_RecvReqS :: "nat \<Rightarrow> nat \<Rightarrow> rule" where
   "n_RecvReqS N i \<equiv>
@@ -448,40 +272,25 @@ definition n_RecvReqS :: "nat \<Rightarrow> nat \<Rightarrow> rule" where
     assign (Para ''Chan1.Cmd'' i, Const Empty) ||
     forallStm (\<lambda>j. assign (Para ''InvSet'' j, IVar (Para ''ShrSet'' j))) N"
 
-lemma symRecvReqS:
+definition n_RecvReqS_abs :: "nat \<Rightarrow> rule" where
+  "n_RecvReqS_abs M \<equiv>
+    IVar (Ident ''CurCmd'') =\<^sub>f Const Empty
+   \<triangleright>
+    assign (Ident ''CurCmd'', Const ReqS) ||
+    assign (Ident ''CurPtr'', Const (index (M+1))) ||
+    forallStm (\<lambda>j. assign (Para ''InvSet'' j, IVar (Para ''ShrSet'' j))) M"
+
+lemma wellFormedRecvReqS:
   "symParamRule N (n_RecvReqS N)"
+  "wellFormedStatement N (act (n_RecvReqS N i))"
   unfolding n_RecvReqS_def
-  apply (rule symParamRuleI)
-  subgoal unfolding symParamForm_def by auto
-  subgoal apply (auto intro!: symParamStatementParallel symParamStatementForall)
-    unfolding symParamStatement_def symParamStatement2_def mutualDiffVars_def by auto
-  done  
+  apply (auto intro!: symParamRuleI symParamStatementParallel symParamStatementForall)
+  unfolding symParamForm_def symParamStatement_def symParamStatement2_def mutualDiffVars_def by auto
 
 lemma absRecvReqS:
-  "absTransfForm M (pre (n_RecvReqS N i)) =
-    (if i > M then
-       IVar (Ident ''CurCmd'') =\<^sub>f Const Empty
-     else
-       IVar (Ident ''CurCmd'') =\<^sub>f Const Empty \<and>\<^sub>f
-     IVar (Para ''Chan1.Cmd'' i) =\<^sub>f Const ReqS)"
-  unfolding n_RecvReqS_def by auto
-
-lemma absRecvReqSAct:
-  "absTransfStatement2 M (act (n_RecvReqS N i)) =
-    (if i > M then
-       assign (Ident ''CurCmd'', Const ReqS) ||
-       assign (Ident ''CurPtr'', Const (index (M+1))) ||
-       forallStm (\<lambda>j. assign (Para ''InvSet'' j, IVar (Para ''ShrSet'' j))) M
-     else
-       assign (Ident ''CurCmd'', Const ReqS) ||
-       assign (Ident ''CurPtr'', Const (index i)) ||
-       assign (Para ''Chan1.Cmd'' i, Const Empty) ||
-       forallStm (\<lambda>j. assign (Para ''InvSet'' j, IVar (Para ''ShrSet'' j))) M)"
-  unfolding n_RecvReqS_def by auto
-
-lemma RecvReqSWellForm:
-  "wellFormedStatement N (act (n_RecvReqS N i))"
-  unfolding n_RecvReqS_def by auto
+  "absTransfRule M (n_RecvReqS N i) =
+    (if i \<le> M then n_RecvReqS M i else n_RecvReqS_abs M)"
+  unfolding n_RecvReqS_def n_RecvReqS_abs_def by auto
 
 definition n_SendReqE1 :: "nat \<Rightarrow> rule" where
   "n_SendReqE1 i \<equiv>
@@ -490,30 +299,11 @@ definition n_SendReqE1 :: "nat \<Rightarrow> rule" where
    \<triangleright>
     assign (Para ''Chan1.Cmd'' i, Const ReqE)"
 
-lemma symSendReqE1:
+lemma SendReqE1:
   "symParamRule N n_SendReqE1"
-  unfolding n_SendReqE1_def symParamRule_def by auto
-
-lemma absSendReqE1:
-  "absTransfForm M (pre (n_SendReqE1 i)) =
-    (if i > M then
-       dontCareForm
-     else
-       IVar (Para ''Chan1.Cmd'' i) =\<^sub>f Const Empty \<and>\<^sub>f
-       IVar (Para ''Cache.State'' i) =\<^sub>f Const I)"
-  unfolding n_SendReqE1_def by auto
-
-lemma absSendReqE1Act:
-  "absTransfStatement2 M (act (n_SendReqE1 i)) =
-    (if i > M then
-       skip
-     else
-       assign (Para ''Chan1.Cmd'' i, Const ReqE))"
-  unfolding n_SendReqE1_def by auto
-
-lemma SendReqE1WellForm:
   "wellFormedStatement N (act (n_SendReqE1 i))"
-  unfolding n_SendReqE1_def by auto
+  "absTransfRule M (n_SendReqE1 i) = (if i \<le> M then n_SendReqE1 i else chaos \<triangleright> skip)"
+  unfolding n_SendReqE1_def symParamRule_def by auto
 
 definition n_SendReqE2 :: "nat \<Rightarrow> rule" where
   "n_SendReqE2 i \<equiv>
@@ -522,30 +312,11 @@ definition n_SendReqE2 :: "nat \<Rightarrow> rule" where
    \<triangleright>
     assign (Para ''Chan1.Cmd'' i, Const ReqE)"
 
-lemma symSendReqE2:
+lemma SendReqE2:
   "symParamRule N n_SendReqE2"
-  unfolding n_SendReqE2_def symParamRule_def by auto
-
-lemma absSendReqE2:
-  "absTransfForm M (pre (n_SendReqE2 i)) =
-    (if i > M then
-       dontCareForm
-     else
-       IVar (Para ''Chan1.Cmd'' i) =\<^sub>f Const Empty \<and>\<^sub>f
-       IVar (Para ''Cache.State'' i) =\<^sub>f Const S)"
-  unfolding n_SendReqE2_def by auto
-
-lemma absSendReqE2Act:
-  "absTransfStatement2 M (act (n_SendReqE2 i)) =
-    (if i > M then
-       skip
-     else
-       assign (Para ''Chan1.Cmd'' i, Const ReqE))"
-  unfolding n_SendReqE2_def by auto
-
-lemma SendReqE2WellForm:
   "wellFormedStatement N (act (n_SendReqE2 i))"
-  unfolding n_SendReqE2_def by auto
+  "absTransfRule M (n_SendReqE2 i) = (if i \<le> M then n_SendReqE2 i else chaos \<triangleright> skip)"
+  unfolding n_SendReqE2_def symParamRule_def by auto
 
 definition n_SendReqS :: "nat \<Rightarrow> rule" where
   "n_SendReqS i \<equiv>
@@ -556,28 +327,9 @@ definition n_SendReqS :: "nat \<Rightarrow> rule" where
 
 lemma symSendReqS:
   "symParamRule N n_SendReqS"
-  unfolding n_SendReqS_def symParamRule_def by auto 
-
-lemma absSendReqS:
-  "absTransfForm M (pre (n_SendReqS i)) =
-    (if i > M then
-       dontCareForm
-     else
-       IVar (Para ''Chan1.Cmd'' i) =\<^sub>f Const Empty \<and>\<^sub>f
-       IVar (Para ''Cache.State'' i) =\<^sub>f Const I)"
-  unfolding n_SendReqS_def by auto
-
-lemma absSendReqSAct:
-  "absTransfStatement2 M (act (n_SendReqS i)) =
-    (if i > M then
-       skip
-     else
-       assign (Para ''Chan1.Cmd'' i, Const ReqS))"
-  unfolding n_SendReqS_def by auto
-
-lemma SendReqSWellForm:
   "wellFormedStatement N (act (n_SendReqS i))"
-  unfolding n_SendReqS_def by auto
+  "absTransfRule M (n_SendReqS i) = (if i \<le> M then n_SendReqS i else chaos \<triangleright> skip)"
+  unfolding n_SendReqS_def symParamRule_def by auto 
 
 definition rules :: "nat \<Rightarrow> rule set" where
   "rules N \<equiv> {r.
@@ -673,25 +425,30 @@ definition n_RecvInvAck1'_ref :: "nat \<Rightarrow> nat \<Rightarrow> rule" wher
     assign (Para ''ShrSet'' i, Const false) ||
     assign (Ident ''ExGntd'', Const false)"
 
+definition n_RecvInvAck1'_abs :: "nat \<Rightarrow> rule" where
+  "n_RecvInvAck1'_abs M \<equiv>
+    (\<not>\<^sub>f IVar (Ident ''CurCmd'') =\<^sub>f Const Empty \<and>\<^sub>f
+     IVar (Ident ''ExGntd'') =\<^sub>f Const true) \<and>\<^sub>f
+    forallForm (\<lambda>j. \<not>\<^sub>f IVar (Para ''Cache.State'' j) =\<^sub>f Const E) M \<and>\<^sub>f
+    forallForm (\<lambda>j. \<not>\<^sub>f IVar (Para ''Chan2.Cmd'' j) =\<^sub>f Const GntE) M \<and>\<^sub>f
+    forallForm (\<lambda>j. \<not>\<^sub>f IVar (Para ''Chan3.Cmd'' j) =\<^sub>f Const InvAck) M
+   \<triangleright>
+    assign (Ident ''ExGntd'', Const false)"
+
 lemma n_RecvInvAck1'Eq:
   "n_RecvInvAck1' N i = n_RecvInvAck1'_ref N i"
   by (auto simp add: n_RecvInvAck1'_def invAux_def n_RecvInvAck1_def n_RecvInvAck1'_ref_def)
 
-lemma absRecvInvAck1':
-  assumes "M \<le> N"
-  shows
-  "absTransfForm M (pre (n_RecvInvAck1'_ref N i)) =
-    (if i > M then
-       (\<not>\<^sub>f IVar (Ident ''CurCmd'') =\<^sub>f Const Empty \<and>\<^sub>f
-        IVar (Ident ''ExGntd'') =\<^sub>f Const true) \<and>\<^sub>f
-       (\<forall>\<^sub>fj. \<not>\<^sub>f IVar (Para ''Cache.State'' j) =\<^sub>f Const E) M \<and>\<^sub>f
-       (\<forall>\<^sub>fj. \<not>\<^sub>f IVar (Para ''Chan2.Cmd'' j) =\<^sub>f Const GntE) M \<and>\<^sub>f
-       (\<forall>\<^sub>fj. \<not>\<^sub>f IVar (Para ''Chan3.Cmd'' j) =\<^sub>f Const InvAck) M
-     else
-       IVar (Para ''Chan3.Cmd'' i) =\<^sub>f Const InvAck \<and>\<^sub>f
-       \<not>\<^sub>f IVar (Ident ''CurCmd'') =\<^sub>f Const Empty \<and>\<^sub>f
-       IVar (Ident ''ExGntd'') =\<^sub>f Const true)"
-  unfolding n_RecvInvAck1'_ref_def using assms by auto
+lemma wellFormedSendReqE2:
+  "symParamRule N (n_RecvInvAck1'_ref N)"
+  "wellFormedStatement N (act (n_RecvInvAck1'_ref N i))"
+  unfolding n_RecvInvAck1'_ref_def
+  apply (auto intro!: symParamRuleI symParamFormAnd symParamFormForallExcl)
+  unfolding symParamForm_def symParamForm2_def symParamStatement_def by auto
 
+lemma absRecvInvAck1'b:
+  "M \<le> N \<Longrightarrow> absTransfRule M (n_RecvInvAck1'_ref N i) =
+    (if i \<le> M then n_RecvInvAck1 i else n_RecvInvAck1'_abs M)"
+  unfolding n_RecvInvAck1_def n_RecvInvAck1'_ref_def n_RecvInvAck1'_abs_def by auto
 
 end
